tls_wrapper.dfy
@@ -4,6 +4,8 @@ module tls_wrapper {
     import opened Structs
     method tls_opts_create(path : string)
     {
+        var opts := new tls_opts;
+        
 
     }
 }
